

# TECHNIQUES OF INTEGRATION

## Basic Integration Formulas

$$1. \int du = u + C$$

$$2. \int k du = ku + C \quad (\text{any number } k)$$

$$3. \int (du + dv) = \int du + \int dv$$

$$4. \int u^n du = \frac{u^{n+1}}{n+1} + C \quad (n \neq -1)$$

$$5. \int \frac{du}{u} = \ln |u| + C$$

$$6. \int \sin u du = -\cos u + C$$

$$7. \int \cos u du = \sin u + C$$

$$8. \int \sec^2 u du = \tan u + C$$

$$9. \int \csc^2 u du = -\cot u + C$$

$$10. \int \sec u \tan u du = \sec u + C$$

$$11. \int \csc u \cot u du = -\csc u + C$$

$$12. \int \tan u du = -\ln |\cos u| + C \\ = \ln |\sec u| + C$$

$$\begin{aligned} 13. \int \cot u \, du &= \ln |\sin u| + C \\ &= -\ln |\csc u| + C \end{aligned}$$

$$14. \int e^u \, du = e^u + C$$

$$15. \int a^u \, du = \frac{a^u}{\ln a} + C \quad (a > 0, a \neq 1)$$

$$16. \int \sinh u \, du = \cosh u + C$$

$$17. \int \cosh u \, du = \sinh u + C$$

$$18. \int \frac{du}{\sqrt{a^2 - u^2}} = \sin^{-1} \left( \frac{u}{a} \right) + C$$

$$19. \int \frac{du}{a^2 + u^2} = \frac{1}{a} \tan^{-1} \left( \frac{u}{a} \right) + C$$

$$20. \int \frac{du}{u\sqrt{u^2 - a^2}} = \frac{1}{a} \sec^{-1} \left| \frac{u}{a} \right| + C$$

$$21. \int \frac{du}{\sqrt{a^2 + u^2}} = \sinh^{-1} \left( \frac{u}{a} \right) + C \quad (a > 0)$$

$$22. \int \frac{du}{\sqrt{u^2 - a^2}} = \cosh^{-1} \left( \frac{u}{a} \right) + C \quad (u > a > 0)$$

## EXAMPLE 1 Making a Simplifying Substitution

Evaluate

$$\int \frac{2x - 9}{\sqrt{x^2 - 9x + 1}} dx.$$

**Solution**

$$\begin{aligned}\int \frac{2x - 9}{\sqrt{x^2 - 9x + 1}} dx &= \int \frac{du}{\sqrt{u}} \\ &= \int u^{-1/2} du \\ &= \frac{u^{(-1/2)+1}}{(-1/2) + 1} + C \\ &= 2u^{1/2} + C \\ &= 2\sqrt{x^2 - 9x + 1} + C\end{aligned}$$

$$\begin{aligned}u &= x^2 - 9x + 1, \\ du &= (2x - 9) dx.\end{aligned}$$

Table 8.1 Formula 4,  
with  $n = -1/2$



## EXAMPLE 2 Completing the Square

Evaluate

$$\int \frac{dx}{\sqrt{8x - x^2}}.$$

**Solution** We complete the square to simplify the denominator:

$$\begin{aligned} 8x - x^2 &= -(x^2 - 8x) = -(x^2 - 8x + 16 - 16) \\ &= -(x^2 - 8x + 16) + 16 = 16 - (x - 4)^2. \end{aligned}$$

Then

$$\begin{aligned} \int \frac{dx}{\sqrt{8x - x^2}} &= \int \frac{dx}{\sqrt{16 - (x - 4)^2}} \\ &= \int \frac{du}{\sqrt{a^2 - u^2}} \end{aligned}$$

$a = 4, u = (x - 4),$   
 $du = dx$

$$= \sin^{-1} \left( \frac{u}{a} \right) + C$$

Table 8.1, Formula 18

$$= \sin^{-1} \left( \frac{x-4}{4} \right) + C.$$



### EXAMPLE 3 Expanding a Power and Using a Trigonometric Identity

Evaluate

$$\int (\sec x + \tan x)^2 dx.$$

**Solution** We expand the integrand and get

$$(\sec x + \tan x)^2 = \sec^2 x + 2 \sec x \tan x + \tan^2 x.$$

The first two terms on the right-hand side of this equation are familiar; we can integrate them at once. How about  $\tan^2 x$ ? There is an identity that connects it with  $\sec^2 x$ :

$$\tan^2 x + 1 = \sec^2 x, \quad \tan^2 x = \sec^2 x - 1.$$

We replace  $\tan^2 x$  by  $\sec^2 x - 1$  and get

$$\begin{aligned} \int (\sec x + \tan x)^2 dx &= \int (\sec^2 x + 2 \sec x \tan x + \sec^2 x - 1) dx \\ &= 2 \int \sec^2 x dx + 2 \int \sec x \tan x dx - \int 1 dx \\ &= 2 \tan x + 2 \sec x - x + C. \end{aligned}$$



#### EXAMPLE 4     Eliminating a Square Root

Evaluate

$$\int_0^{\pi/4} \sqrt{1 + \cos 4x} \, dx.$$

**Solution**     We use the identity

$$\cos^2 \theta = \frac{1 + \cos 2\theta}{2}, \quad \text{or} \quad 1 + \cos 2\theta = 2 \cos^2 \theta.$$

With  $\theta = 2x$ , this identity becomes

$$1 + \cos 4x = 2 \cos^2 2x.$$

Hence,

$$\int_0^{\pi/4} \sqrt{1 + \cos 4x} \, dx = \int_0^{\pi/4} \sqrt{2} \sqrt{\cos^2 2x} \, dx$$



$$= \sqrt{2} \int_0^{\pi/4} |\cos 2x| \, dx$$

$$\sqrt{u^2} = |u|$$

$$= \sqrt{2} \int_0^{\pi/4} \cos 2x \, dx$$

On  $[0, \pi/4]$ ,  $\cos 2x \geq 0$ ,  
so  $|\cos 2x| = \cos 2x$ .

$$= \sqrt{2} \left[ \frac{\sin 2x}{2} \right]_0^{\pi/4}$$

Table 8.1, Formula 7, with  
 $u = 2x$  and  $du = 2 \, dx$

$$= \sqrt{2} \left[ \frac{1}{2} - 0 \right] = \frac{\sqrt{2}}{2}.$$



## EXAMPLE 5 Reducing an Improper Fraction

Evaluate

$$\int \frac{3x^2 - 7x}{3x + 2} \, dx.$$

**Solution** The integrand is an improper fraction (degree of numerator greater than or equal to degree of denominator). To integrate it, we divide first, getting a quotient plus a remainder that is a proper fraction:

$$\begin{array}{r}
 \overline{) 3x + 2 \over 3x^2 - 7x} \\
 \underline{3x^2 + 2x} \phantom{0} \\
 -9x \phantom{0} \\
 \underline{-9x - 6} \\
 + 6
 \end{array}$$

$$\frac{3x^2 - 7x}{3x + 2} = x - 3 + \frac{6}{3x + 2}.$$

Therefore,

$$\int \frac{3x^2 - 7x}{3x + 2} dx = \int \left( x - 3 + \frac{6}{3x + 2} \right) dx = \frac{x^2}{2} - 3x + 2 \ln |3x + 2| + C. \quad \blacksquare$$

## EXAMPLE 6     Separating a Fraction

Evaluate

$$\int \frac{3x + 2}{\sqrt{1 - x^2}} dx.$$

**Solution**     We first separate the integrand to get

$$\int \frac{3x + 2}{\sqrt{1 - x^2}} dx = 3 \int \frac{x dx}{\sqrt{1 - x^2}} + 2 \int \frac{dx}{\sqrt{1 - x^2}}.$$

In the first of these new integrals, we substitute

$$u = 1 - x^2, \quad du = -2x dx, \quad \text{and} \quad x dx = -\frac{1}{2} du.$$

$$\begin{aligned} 3 \int \frac{x \, dx}{\sqrt{1-x^2}} &= 3 \int \frac{(-1/2) \, du}{\sqrt{u}} = -\frac{3}{2} \int u^{-1/2} \, du \\ &= -\frac{3}{2} \cdot \frac{u^{1/2}}{1/2} + C_1 = -3\sqrt{1-x^2} + C_1 \end{aligned}$$

The second of the new integrals is a standard form,

$$2 \int \frac{dx}{\sqrt{1-x^2}} = 2 \sin^{-1} x + C_2.$$

Combining these results and renaming  $C_1 + C_2$  as  $C$  gives

$$\int \frac{3x+2}{\sqrt{1-x^2}} \, dx = -3\sqrt{1-x^2} + 2 \sin^{-1} x + C.$$



**EXAMPLE 7** Integral of  $y = \sec x$ —Multiplying by a Form of 1

Evaluate

$$\int \sec x \, dx.$$

**Solution**

$$\begin{aligned}\int \sec x \, dx &= \int (\sec x)(1) \, dx = \int \sec x \cdot \frac{\sec x + \tan x}{\sec x + \tan x} \, dx \\&= \int \frac{\sec^2 x + \sec x \tan x}{\sec x + \tan x} \, dx \\&= \int \frac{du}{u} \\&= \ln |u| + C = \ln |\sec x + \tan x| + C.\end{aligned}$$

$$\begin{aligned}u &= \tan x + \sec x, \\du &= (\sec^2 x + \sec x \tan x) \, dx\end{aligned}$$



**TABLE 8.2** The secant and cosecant integrals

---

1.  $\int \sec u \, du = \ln |\sec u + \tan u| + C$

2.  $\int \csc u \, du = -\ln |\csc u + \cot u| + C$

## Integration by Parts

$$\int f(x)g'(x) dx = f(x)g(x) - \int f'(x)g(x) dx \quad (1)$$

$$\int u dv = uv - \int v du \quad (2)$$

## EXAMPLE 1 Using Integration by Parts

Find

$$\int x \cos x \, dx.$$

**Solution** We use the formula  $\int u \, dv = uv - \int v \, du$  with

$$\begin{aligned} u &= x, & dv &= \cos x \, dx, \\ du &= dx, & v &= \sin x. \end{aligned}$$

Simplest antiderivative of  $\cos x$

Then

$$\int x \cos x \, dx = x \sin x - \int \sin x \, dx = x \sin x + \cos x + C.$$





## EXAMPLE

Find

$$\int \ln x \, dx.$$

**Solution** Since  $\int \ln x \, dx$  can be written as  $\int \ln x \cdot 1 \, dx$ , we use the formula  $\int u \, dv = uv - \int v \, du$  with

$$u = \ln x \quad \text{Simplifies when differentiated}$$

$$dv = dx \quad \text{Easy to integrate}$$

$$du = \frac{1}{x} dx,$$

$$v = x. \quad \text{Simplest antiderivative}$$

Then

$$\int \ln x \, dx = x \ln x - \int x \cdot \frac{1}{x} dx = x \ln x - \int dx = x \ln x - x + C. \quad \blacksquare$$

## EXAMPLE

Evaluate

$$\int x^2 e^x dx.$$

**Solution** With  $u = x^2$ ,  $dv = e^x dx$ ,  $du = 2x dx$ , and  $v = e^x$ , we have

$$\int x^2 e^x dx = x^2 e^x - 2 \int x e^x dx.$$

The new integral is less complicated than the original because the exponent on  $x$  is reduced by one. To evaluate the integral on the right, we integrate by parts again with  $u = x$ ,  $dv = e^x dx$ . Then  $du = dx$ ,  $v = e^x$ , and

$$\int x e^x dx = x e^x - \int e^x dx = x e^x - e^x + C.$$

Hence,

$$\begin{aligned}\int x^2 e^x dx &= x^2 e^x - 2 \int x e^x dx \\ &= x^2 e^x - 2x e^x + 2e^x + C.\end{aligned}$$

### EXAMPLE

Evaluate

$$\int e^x \cos x dx.$$

**Solution** Let  $u = e^x$  and  $dv = \cos x dx$ . Then  $du = e^x dx$ ,  $v = \sin x$ , and

$$\int e^x \cos x dx = e^x \sin x - \int e^x \sin x dx.$$

The second integral is like the first except that it has  $\sin x$  in place of  $\cos x$ . To evaluate it, we use integration by parts with

$$u = e^x, \quad dv = \sin x \, dx, \quad v = -\cos x, \quad du = e^x \, dx.$$

Then

$$\begin{aligned} \int e^x \cos x \, dx &= e^x \sin x - \left( -e^x \cos x - \int (-\cos x)(e^x \, dx) \right) \\ &= e^x \sin x + e^x \cos x - \int e^x \cos x \, dx. \end{aligned}$$

The unknown integral now appears on both sides of the equation. Adding the integral to both sides and adding the constant of integration gives

$$2 \int e^x \cos x \, dx = e^x \sin x + e^x \cos x + C_1.$$

Dividing by 2 and renaming the constant of integration gives

$$\int e^x \cos x \, dx = \frac{e^x \sin x + e^x \cos x}{2} + C.$$



### Integration by Parts Formula for Definite Integrals

$$\int_a^b f(x)g'(x) \, dx = f(x)g(x) \Big|_a^b - \int_a^b f'(x)g(x) \, dx \quad (3)$$

### EXAMPLE

Find the area of the region bounded by the curve  $y = xe^{-x}$  and the  $x$ -axis from  $x = 0$  to  $x = 4$ .

**Solution** The region is shaded in Figure 8.1. Its area is

$$\int_0^4 xe^{-x} dx.$$

Let  $u = x$ ,  $dv = e^{-x} dx$ ,  $v = -e^{-x}$ , and  $du = dx$ . Then,

$$\begin{aligned}\int_0^4 xe^{-x} dx &= -xe^{-x} \Big|_0^4 - \int_0^4 (-e^{-x}) dx \\&= [-4e^{-4} - (0)] + \int_0^4 e^{-x} dx \\&= -4e^{-4} - e^{-x} \Big|_0^4 \\&= -4e^{-4} - e^{-4} - (-e^0) = 1 - 5e^{-4} \approx 0.91.\end{aligned}$$



## EXAMPLE Using Tabular Integration

Evaluate

$$\int x^2 e^x dx.$$

**Solution** With  $f(x) = x^2$  and  $g(x) = e^x$ , we list:

---

**$f(x)$  and its derivatives**

**$g(x)$  and its integrals**

---

$x^2$	$(+)$	$e^x$
$2x$	$(-)$	$e^x$
$2$	$(+)$	$e^x$
$0$		$e^x$

---

We combine the products of the functions connected by the arrows according to the operation signs above the arrows to obtain

$$\int x^2 e^x dx = x^2 e^x - 2x e^x + 2e^x + C.$$

### EXAMPLE

Evaluate

$$\int x^3 \sin x dx.$$



**Solution**

With  $f(x) = x^3$  and  $g(x) = \sin x$ , we list:

$f(x)$ and its derivatives		$g(x)$ and its integrals
$x^3$	$(+)$	$\sin x$
$3x^2$	$(-)$	$-\cos x$
$6x$	$(+)$	$-\sin x$
$6$	$(-)$	$\cos x$
$0$		$\sin x$

Again we combine the products of the functions connected by the arrows according to the operation signs above the arrows to obtain

$$\int x^3 \sin x \, dx = -x^3 \cos x + 3x^2 \sin x + 6x \cos x - 6 \sin x + C. \quad \blacksquare$$

# Integration of Rational Functions by Partial Fractions

The method for rewriting rational functions as a sum of simpler fractions is called **the method of partial fractions**. In the case of the above example, it consists of finding constants  $A$  and  $B$  such that

$$\frac{5x - 3}{x^2 - 2x - 3} = \frac{A}{x + 1} + \frac{B}{x - 3}. \quad (1)$$

(Pretend for a moment that we do not know that  $A = 2$  and  $B = 3$  will work.) We call the fractions  $A/(x + 1)$  and  $B/(x - 3)$  **partial fractions** because their denominators are only part of the original denominator  $x^2 - 2x - 3$ . We call  $A$  and  $B$  **undetermined coefficients** until proper values for them have been found.

To find  $A$  and  $B$ , we first clear Equation (1) of fractions, obtaining

$$5x - 3 = A(x - 3) + B(x + 1) = (A + B)x - 3A + B.$$

This will be an identity in  $x$  if and only if the coefficients of like powers of  $x$  on the two sides are equal:

$$A + B = 5, \quad -3A + B = -3.$$

Solving these equations simultaneously gives  $A = 2$  and  $B = 3$ .

## Method of Partial Fractions ( $f(x)/g(x)$ Proper)

1. Let  $x - r$  be a linear factor of  $g(x)$ . Suppose that  $(x - r)^m$  is the highest power of  $x - r$  that divides  $g(x)$ . Then, to this factor, assign the sum of the  $m$  partial fractions:

$$\frac{A_1}{x - r} + \frac{A_2}{(x - r)^2} + \cdots + \frac{A_m}{(x - r)^m}.$$

Do this for each distinct linear factor of  $g(x)$ .

2. Let  $x^2 + px + q$  be a quadratic factor of  $g(x)$ . Suppose that  $(x^2 + px + q)^n$  is the highest power of this factor that divides  $g(x)$ . Then, to this factor, assign the sum of the  $n$  partial fractions:

$$\frac{B_1x + C_1}{x^2 + px + q} + \frac{B_2x + C_2}{(x^2 + px + q)^2} + \cdots + \frac{B_nx + C_n}{(x^2 + px + q)^n}.$$

Do this for each distinct quadratic factor of  $g(x)$  that cannot be factored into linear factors with real coefficients.

3. Set the original fraction  $f(x)/g(x)$  equal to the sum of all these partial fractions. Clear the resulting equation of fractions and arrange the terms in decreasing powers of  $x$ .
4. Equate the coefficients of corresponding powers of  $x$  and solve the resulting equations for the undetermined coefficients.

### EXAMPLE 1 Distinct Linear Factors

Evaluate

$$\int \frac{x^2 + 4x + 1}{(x - 1)(x + 1)(x + 3)} dx$$

using partial fractions.

**Solution** The partial fraction decomposition has the form

$$\frac{x^2 + 4x + 1}{(x - 1)(x + 1)(x + 3)} = \frac{A}{x - 1} + \frac{B}{x + 1} + \frac{C}{x + 3}.$$

To find the values of the undetermined coefficients  $A$ ,  $B$ , and  $C$  we clear fractions and get

$$\begin{aligned} x^2 + 4x + 1 &= A(x + 1)(x + 3) + B(x - 1)(x + 3) + C(x - 1)(x + 1) \\ &= (A + B + C)x^2 + (4A + 2B)x + (3A - 3B - C). \end{aligned}$$

The polynomials on both sides of the above equation are identical, so we equate coefficients of like powers of  $x$  obtaining

$$\text{Coefficient of } x^2: \quad A + B + C = 1$$

$$\text{Coefficient of } x^1: \quad 4A + 2B = 4$$

$$\text{Coefficient of } x^0: \quad 3A - 3B - C = 1$$

There are several ways for solving such a system of linear equations for the unknowns  $A$ ,  $B$ , and  $C$ , including elimination of variables, or the use of a calculator or computer. Whatever method is used, the solution is  $A = 3/4$ ,  $B = 1/2$ , and  $C = -1/4$ . Hence we have

$$\begin{aligned} \int \frac{x^2 + 4x + 1}{(x - 1)(x + 1)(x + 3)} dx &= \int \left[ \frac{3}{4} \frac{1}{x - 1} + \frac{1}{2} \frac{1}{x + 1} - \frac{1}{4} \frac{1}{x + 3} \right] dx \\ &= \frac{3}{4} \ln |x - 1| + \frac{1}{2} \ln |x + 1| - \frac{1}{4} \ln |x + 3| + K, \end{aligned}$$

where  $K$  is the arbitrary constant of integration (to avoid confusion with the undetermined coefficient we labeled as  $C$ ). ■



## EXAMPLE 2     A Repeated Linear Factor

Evaluate

$$\int \frac{6x + 7}{(x + 2)^2} dx.$$

**Solution**     First we express the integrand as a sum of partial fractions with undetermined coefficients.

$$\frac{6x + 7}{(x + 2)^2} = \frac{A}{x + 2} + \frac{B}{(x + 2)^2}$$

$$6x + 7 = A(x + 2) + B \quad \text{Multiply both sides by } (x + 2)^2.$$

$$= Ax + (2A + B)$$

Equating coefficients of corresponding powers of  $x$  gives

$$A = 6 \quad \text{and} \quad 2A + B = 12 + B = 7, \quad \text{or} \quad A = 6 \quad \text{and} \quad B = -5.$$

Therefore,

$$\begin{aligned}\int \frac{6x + 7}{(x + 2)^2} dx &= \int \left( \frac{6}{x + 2} - \frac{5}{(x + 2)^2} \right) dx \\ &= 6 \int \frac{dx}{x + 2} - 5 \int (x + 2)^{-2} dx \\ &= 6 \ln |x + 2| + 5(x + 2)^{-1} + C\end{aligned}$$



### EXAMPLE 3 Integrating an Improper Fraction

Evaluate

$$\int \frac{2x^3 - 4x^2 - x - 3}{x^2 - 2x - 3} dx.$$

**Solution** First we divide the denominator into the numerator to get a polynomial plus a proper fraction.

$$\begin{array}{r} 2x \\ x^2 - 2x - 3 \overline{) 2x^3 - 4x^2 - x - 3} \\ \underline{2x^3 - 4x^2 - 6x} \phantom{- 3} \\ 5x - 3 \end{array}$$

Then we write the improper fraction as a polynomial plus a proper fraction.

$$\frac{2x^3 - 4x^2 - x - 3}{x^2 - 2x - 3} = 2x + \frac{5x - 3}{x^2 - 2x - 3}$$

We found the partial fraction decomposition of the fraction on the right in the opening example, so

$$\begin{aligned} \int \frac{2x^3 - 4x^2 - x - 3}{x^2 - 2x - 3} dx &= \int 2x dx + \int \frac{5x - 3}{x^2 - 2x - 3} dx \\ &= \int 2x dx + \int \frac{2}{x + 1} dx + \int \frac{3}{x - 3} dx \\ &= x^2 + 2 \ln |x + 1| + 3 \ln |x - 3| + C. \end{aligned}$$



## EXAMPLE 4

Evaluate

$$\int \frac{-2x + 4}{(x^2 + 1)(x - 1)^2} dx$$

using partial fractions.

**Solution** The denominator has an irreducible quadratic factor as well as a repeated linear factor, so we write

$$\frac{-2x + 4}{(x^2 + 1)(x - 1)^2} = \frac{Ax + B}{x^2 + 1} + \frac{C}{x - 1} + \frac{D}{(x - 1)^2}. \quad (2)$$

Clearing the equation of fractions gives

$$\begin{aligned} -2x + 4 &= (Ax + B)(x - 1)^2 + C(x - 1)(x^2 + 1) + D(x^2 + 1) \\ &= (A + C)x^3 + (-2A + B - C + D)x^2 \end{aligned}$$

$$+ (A - 2B + C)x + (B - C + D).$$

Equating coefficients of like terms gives

$$\text{Coefficients of } x^3: \quad 0 = A + C$$

$$\text{Coefficients of } x^2: \quad 0 = -2A + B - C + D$$

$$\text{Coefficients of } x^1: \quad -2 = A - 2B + C$$

$$\text{Coefficients of } x^0: \quad 4 = B - C + D$$

We solve these equations simultaneously to find the values of  $A$ ,  $B$ ,  $C$ , and  $D$ :

$$-4 = -2A, \quad A = 2 \quad \text{Subtract fourth equation from second.}$$

$$C = -A = -2 \quad \text{From the first equation}$$

$$B = 1 \quad A = 2 \text{ and } C = -2 \text{ in third equation.}$$

$$D = 4 - B + C = 1. \quad \text{From the fourth equation}$$

We substitute these values into Equation (2), obtaining

$$\frac{-2x + 4}{(x^2 + 1)(x - 1)^2} = \frac{2x + 1}{x^2 + 1} - \frac{2}{x - 1} + \frac{1}{(x - 1)^2}.$$

Finally, using the expansion above we can integrate:

$$\begin{aligned}\int \frac{-2x + 4}{(x^2 + 1)(x - 1)^2} dx &= \int \left( \frac{2x + 1}{x^2 + 1} - \frac{2}{x - 1} + \frac{1}{(x - 1)^2} \right) dx \\ &= \int \left( \frac{2x}{x^2 + 1} + \frac{1}{x^2 + 1} - \frac{2}{x - 1} + \frac{1}{(x - 1)^2} \right) dx \\ &= \ln(x^2 + 1) + \tan^{-1} x - 2 \ln |x - 1| - \frac{1}{x - 1} + C. \quad \blacksquare\end{aligned}$$

### EXAMPLE 5     A Repeated Irreducible Quadratic Factor

Evaluate

$$\int \frac{dx}{x(x^2 + 1)^2}.$$

**Solution**     The form of the partial fraction decomposition is

$$\frac{1}{x(x^2 + 1)^2} = \frac{A}{x} + \frac{Bx + C}{x^2 + 1} + \frac{Dx + E}{(x^2 + 1)^2}$$

Multiplying by  $x(x^2 + 1)^2$ , we have

$$\begin{aligned} 1 &= A(x^2 + 1)^2 + (Bx + C)x(x^2 + 1) + (Dx + E)x \\ &= A(x^4 + 2x^2 + 1) + B(x^4 + x^2) + C(x^3 + x) + Dx^2 + Ex \\ &= (A + B)x^4 + Cx^3 + (2A + B + D)x^2 + (C + E)x + A \end{aligned}$$

If we equate coefficients, we get the system

$$A + B = 0, \quad C = 0, \quad 2A + B + D = 0, \quad C + E = 0, \quad A = 1.$$

Solving this system gives  $A = 1$ ,  $B = -1$ ,  $C = 0$ ,  $D = -1$ , and  $E = 0$ . Thus,

$$\begin{aligned} \int \frac{dx}{x(x^2 + 1)^2} &= \int \left[ \frac{1}{x} + \frac{-x}{x^2 + 1} + \frac{-x}{(x^2 + 1)^2} \right] dx \\ &= \int \frac{dx}{x} - \int \frac{x dx}{x^2 + 1} - \int \frac{x dx}{(x^2 + 1)^2} \\ &= \int \frac{dx}{x} - \frac{1}{2} \int \frac{du}{u} - \frac{1}{2} \int \frac{du}{u^2} && \begin{array}{l} u = x^2 + 1, \\ du = 2x dx \end{array} \\ &= \ln |x| - \frac{1}{2} \ln |u| + \frac{1}{2u} + K \\ &= \ln |x| - \frac{1}{2} \ln (x^2 + 1) + \frac{1}{2(x^2 + 1)} + K \\ &= \ln \frac{|x|}{\sqrt{x^2 + 1}} + \frac{1}{2(x^2 + 1)} + K. \end{aligned}$$





$$17. \int_0^1 \frac{x^3 dx}{x^2 + 2x + 1}$$

$$\frac{x^3}{x^2 + 2x + 1} = (x - 2) + \frac{3x + 2}{(x + 1)^2} \text{ (after long division);}$$

$$\frac{3x + 2}{(x + 1)^2} = \frac{A}{x + 1} + \frac{B}{(x + 1)^2} \Rightarrow 3x + 2 = A(x + 1) + B$$

$$= Ax + (A + B) \Rightarrow A = 3, A + B = 2 \Rightarrow A = 3, B = -1; \int_0^1 \frac{x^3 dx}{x^2 + 2x + 1}$$

$$= \int_0^1 (x - 2) dx + 3 \int_0^1 \frac{dx}{x + 1} - \int_0^1 \frac{dx}{(x + 1)^2} = \left[ \frac{x^2}{2} - 2x + 3 \ln |x + 1| + \frac{1}{x + 1} \right]_0^1$$


$$= \left( \frac{1}{2} - 2 + 3 \ln 2 + \frac{1}{2} \right) - (1) = 3 \ln 2 - 2$$

# Trigonometric Integrals

**EXAMPLE 1** Evaluate

$$\int \sin^3 x \cos^2 x \, dx.$$

**Solution**

$$\begin{aligned}\int \sin^3 x \cos^2 x \, dx &= \int \sin^2 x \cos^2 x \sin x \, dx \\&= \int (1 - \cos^2 x) \cos^2 x (-d(\cos x)) \\&= \int (1 - u^2)(u^2)(-du) && u = \cos x \\&= \int (u^4 - u^2) \, du \\&= \frac{u^5}{5} - \frac{u^3}{3} + C \\&= \frac{\cos^5 x}{5} - \frac{\cos^3 x}{3} + C.\end{aligned}$$


## EXAMPLE 2

Evaluate

$$\int \cos^5 x \, dx.$$

**Solution**

$$\int \cos^5 x \, dx = \int \cos^4 x \cos x \, dx = \int (1 - \sin^2 x)^2 d(\sin x) \quad m = 0$$

$$= \int (1 - u^2)^2 du \quad u = \sin x$$

$$= \int (1 - 2u^2 + u^4) du$$

$$= u - \frac{2}{3}u^3 + \frac{1}{5}u^5 + C = \sin x - \frac{2}{3}\sin^3 x + \frac{1}{5}\sin^5 x + C. \quad \blacksquare$$

**EXAMPLE 3**  $m$  and  $n$  are Both Even

Evaluate

$$\int \sin^2 x \cos^4 x \, dx.$$

**Solution**

$$\begin{aligned}\int \sin^2 x \cos^4 x \, dx &= \int \left( \frac{1 - \cos 2x}{2} \right) \left( \frac{1 + \cos 2x}{2} \right)^2 dx \\&= \frac{1}{8} \int (1 - \cos 2x)(1 + 2 \cos 2x + \cos^2 2x) \, dx \\&= \frac{1}{8} \int (1 + \cos 2x - \cos^2 2x - \cos^3 2x) \, dx \\&= \frac{1}{8} \left[ x + \frac{1}{2} \sin 2x - \int (\cos^2 2x + \cos^3 2x) \, dx \right].\end{aligned}$$

For the term involving  $\cos^2 2x$  we use

$$\begin{aligned}\int \cos^2 2x \, dx &= \frac{1}{2} \int (1 + \cos 4x) \, dx \\ &= \frac{1}{2} \left( x + \frac{1}{4} \sin 4x \right).\end{aligned}$$

Omitting the constant of integration until the final result

For the  $\cos^3 2x$  term we have

$$\begin{aligned}\int \cos^3 2x \, dx &= \int (1 - \sin^2 2x) \cos 2x \, dx \\ &= \frac{1}{2} \int (1 - u^2) \, du = \frac{1}{2} \left( \sin 2x - \frac{1}{3} \sin^3 2x \right).\end{aligned}$$

$u = \sin 2x,$   
 $du = 2 \cos 2x \, dx$

Again omitting  $C$

Combining everything and simplifying we get

$$\int \sin^2 x \cos^4 x \, dx = \frac{1}{16} \left( x - \frac{1}{4} \sin 4x + \frac{1}{3} \sin^3 2x \right) + C.$$

